books/evm/memory-defthms.lisp
@@ -1,0 +1,16 @@
+(in-package "ACL2")
+
+(include-book "memory")
+
+(defthm memory-empty-validp
+    (and (memory/validp nil)
+         (memory/validp (mk-empty-memory)))
+  :hints (("Goal"
+           :in-theory (enable memory/validp))))
+
+(defthm memory-load-byte-evm-bytep
+    (implies (memory/validp m)
+             (evm-bytep (memory/load-byte m addr)))
+  :hints (("Goal"
+           :in-theory (enable memory/validp
+                              memory/load-byte))))
